Meeting notes; revive Uninitialized data PCM

examples/steel/arraystructs/IntOrBool.fsti
@@ -12,6 +12,9 @@ module A = Steel.Effect.Atomic
 ///
 /// Carrier of PCM for int_or_bool:
 
+[@@erasable]
+noeq type tag = | I' | B'
+
 val int_or_bool : Type0
 
 /// PCM for int_or_bool:
@@ -21,8 +24,14 @@ val int_or_bool_pcm : refined_one_pcm int_or_bool
 /// (mk_int i) represents (union int_or_bool){.i = i}
 /// (mk_bool b) represents (union int_or_bool){.b = b}
 
-val mk_int (i: Ghost.erased (pod int)): Ghost.erased int_or_bool
-val mk_bool (i: Ghost.erased (pod bool)): Ghost.erased int_or_bool
+let int_or_bool_cases k : Type = match k with
+  | I' -> pod int
+  | B' -> pod bool
+
+val mk: tag -> Ghost.erased (int_or_bool_cases tag) -> Ghost.erased int_or_bool
+
+//val mk_int (i: Ghost.erased (pod int)): Ghost.erased int_or_bool
+//val mk_bool (i: Ghost.erased (pod bool)): Ghost.erased int_or_bool
 
 /// Refinements for cases
 
@@ -35,6 +44,11 @@ val _i : pcm_lens (refined_pcm re_i) (pod_pcm int)
 val _b : pcm_lens (refined_pcm re_b) (pod_pcm bool)
 
 /// Taking pointers to the i and b cases of an int_or_bool
+
+//val addr_of_i (#i: Ghost.erased (pod int){case u == I}) (p: ref 'a int_or_bool_pcm)
+//: SteelT (q:ref 'a (pod_pcm int){q == ref_focus (ref_refine p re_i) _i})
+//    (p `pts_to` u)
+//    (fun q -> q `pts_to` proj2 u)
 
 val addr_of_i (#i: Ghost.erased (pod int)) (p: ref 'a int_or_bool_pcm)
 : SteelT (q:ref 'a (pod_pcm int){q == ref_focus (ref_refine p re_i) _i})
@@ -55,3 +69,43 @@ val unaddr_of_b (#b: Ghost.erased (pod bool)) (#opened: M.inames)
   (p: ref 'a int_or_bool_pcm)
   (q: ref 'a (pod_pcm bool){q == ref_focus (ref_refine p re_b) _b})
 : A.SteelGhostT unit opened (q `pts_to` b) (fun _ -> p `pts_to` mk_bool b)
+
+/// Laws (compare with FStar.PCM.POD.fsti)
+
+val case: Ghost.erased int_or_bool -> GTot (option tag)
+val case_ok1: u:Ghost.erased int_or_bool -> t:tag -> x:typeof_pcm t ->
+  Lemma (case (mk t i) == Some t) [SMTPat (case (mk t i))]
+val case_ok2: u -> Lemma (case u == None <==> u = one _) [SMTPat (case u)]
+val case_ok3: u: _ ->
+  Lemma
+    (requires Some? (case u))
+    (ensures exists i. u == mk (Some?.v (case u)) i) [SMTPat (case u)]
+
+// let is_int_int (i:Ghost.erased (pod int)): Lemma (is_int (mk_int i)) = ()
+// let is_bool_bool (b:Ghost.erased (pod bool)): Lemma (is_bool (mk_bool b)) = ()
+// 
+// let int_not_bool (u: Ghost.erased int_or_bool)
+// : Lemma (requires is_int u) (ensures ~ (is_bool u)) 
+// = ()
+// 
+// let bool_not_int (u: Ghost.erased int_or_bool)
+// : Lemma (requires is_bool u) (ensures ~ (is_int u)) 
+// = ()
+// 
+// val int_compatible (v w: Ghost.erased int_or_bool)
+// : Lemma (requires compatible int_or_bool_pcm v w /\ is_int v) (ensures is_int w)
+//   [SMTPat (compatible int_or_bool_pcm v w); SMTPat (is_int v)]
+// 
+// val bool_compatible (v w: Ghost.erased int_or_bool)
+// : Lemma (requires compatible int_or_bool_pcm v w /\ is_bool v) (ensures is_bool w)
+//   [SMTPat (compatible int_or_bool_pcm v w); SMTPat (is_bool v)]
+//   
+// val int_valid_write (v w: Ghost.erased (pod int))
+// : Lemma
+//     (requires AggregateRef.valid_write (pod_pcm int) v w)
+//     (ensures AggregateRef.valid_write int_or_bool_pcm (mk_int v) (mk_int w))
+//   [SMTPat (AggregateRef.valid_write (pod_pcm int) v w)]
+// 
+// v, w whole
+// I != J
+// valid_write (mk I v) (mk J w) 
