examples/steel/arraystructs/FStar.PCM.POD.fsti
@@ -11,6 +11,8 @@ val some: Ghost.erased 'a -> Ghost.erased (pod 'a)
 val is_some: Ghost.erased (pod 'a) -> prop
 val some_v: x:pod 'a{is_some x} -> GTot (y:'a{x == Ghost.reveal (some y)})
 
+val some': x:'a -> y:pod 'a{y == Ghost.reveal (some x)}
+
 val pod_pcm (a:Type): refined_one_pcm (pod a)
 
 val none_is_unit (a:Type): Lemma (Ghost.reveal none == one (pod_pcm a)) [SMTPat (one (pod_pcm a))]
